Add Queue iterators

src/linear/adt/Queue1.dfy
@@ -98,3 +98,56 @@ class Queue1 extends Queue {
     x := list.PopFront();
   }
 }
+
+class QueueIterator {
+  ghost var index: nat
+  ghost var parent: Queue1
+  var node: Node?
+
+  predicate Valid()
+    reads this, parent, parent.Repr()
+  {
+    && parent.Valid()
+    && ( node != null ==>
+          && node in parent.list.list.Repr()
+          && index == parent.list.list.GetIndex(node)
+      )
+  }
+
+  constructor(l: Queue1)
+    requires l.Valid()
+    ensures Valid()
+    ensures parent == l
+  {
+    index := 0;
+    parent := l;
+    node := l.list.list.head;
+  }
+
+  function method HasNext(): bool
+    reads this
+  {
+    node != null
+  }
+
+  method Next() returns (x: int)
+    modifies this
+    requires HasNext()
+    requires Valid()
+    ensures Valid()
+    ensures x == old(parent.Model()[index])
+    ensures old(index) < index
+    ensures parent == old(parent)
+  {
+    { // GHOST
+      parent.list.list.ModelRelationWithSpine();
+      if index < |parent.list.list.spine|-1 {
+        assert parent.list.list.spine[index+1]
+          == parent.list.list.spine[index].next;
+      }
+    }
+    x := node.data;
+    index := index + 1;
+    node := node.next;
+  }
+}
