src/linear/adt/Queue1.Examples.dfy
@@ -1,0 +1,14 @@
+include "../../../src/linear/adt/Queue1.dfy"
+
+method ItertatorExample() {
+  var q: Queue1 := new Queue1();
+  var it := new QueueIterator(q);
+  while it.HasNext()
+    invariant it.Valid()
+    invariant it.parent == q
+    decreases |q.Model()| - it.index
+  {
+    var x := it.Next();
+    print(x);
+  }
+}
